theories/rules/rules_IsUnique.v
@@ -18,22 +18,6 @@ Section cap_lang_rules.
   Implicit Types mem : Mem.
   Implicit Types lmem : LMem.
 
-
-  (* TODO and version are equals ? *)
-  Definition overlap_lwords (lw1 lw2 : LWord) : Prop :=
-    (overlap_word (lword_get_word lw1) (lword_get_word lw2)) = true.
-
-  (* For all addresses in the given region, update the version of the address *)
-  Definition update_version (lmem : LMem) (region : list Addr) (old_v new_v : Version)
-    : option LMem :=
-    foldl
-      (fun (opt_lmem' : option LMem) (a : Addr) =>
-         lmem' ← opt_lmem';
-         lw ← lmem' !! (a, old_v);
-         Some (<[(a, new_v) := lw ]> lmem'))
-      (Some lmem)
-      region.
-
   Inductive IsUnique_fail (lregs : LReg) (lmem : LMem) (dst src : RegName): Prop :=
   | IsUnique_fail_cap (lwsrc: LWord) :
     lregs !! src = Some lwsrc ->
@@ -51,55 +35,26 @@ Section cap_lang_rules.
     incrementLPC (<[ dst := LInt 0 ]> lregs) = None ->
     IsUnique_fail lregs lmem dst src.
 
+  Definition unique_in_machineL (lmem : LMem) (lregs : LReg) (src : RegName)
+    (lwsrc : LWord) : Prop . Admitted.
+  Definition update_version_word_region (lmem : LMem) (lwsrc : LWord)
+    (v : Version) : option LMem. Admitted.
 
-  (* TODO move *)
-  Definition unique_in_memoryL (lmem : LMem) (lwsrc : LWord) (v : Version) : Prop :=
-    Forall
-      (fun (la : LAddr) =>
-         match lmem !! la with
-         | None => True
-         | Some lw => not (overlap_lwords lwsrc lw)
-         end)
-      (logical_region all_memory v).
-
-  Definition unique_in_registersL  (lregs : LReg) (lwsrc : LWord) (src : RegName) : Prop :=
-    Forall
-      (fun (r : RegName) =>
-         match lregs !! r with
-         | None => True
-         | Some lw => r <> src -> not (overlap_lwords lwsrc lw)
-         end)
-      all_registers.
-
-  Definition unique_in_machineL (lregs : LReg) (lmem : LMem)
-    (lwsrc : LWord) (src : RegName) (v : Version) : Prop :=
-    ( forall (full_lregs : LReg) (full_lmem : LMem),
-        (* NOTE We need to consider any /compatible/ logical registers/memory
-           such that, the given logical state in included in. This way, although we
-           are working on a local view, the sweep is over any bigger
-           logical register/memory. *)
-        lregs ⊆ full_lregs ->
-        lmem ⊆ full_lmem ->
-        unique_in_memoryL full_lmem lwsrc v /\ unique_in_registersL full_lregs lwsrc src).
-
-  (* TODO lemmas to express [unique_in_*L] in terms of [unique_in_*] *)
-
-  Lemma unique_in_machineL_weaken
-    (lregs lregs' : LReg) (lmem lmem' : LMem)
-    (lwsrc : LWord) (src : RegName) (v : Version) :
-    lregs' ⊆ lregs ->
-    lmem' ⊆ lmem ->
-    unique_in_machineL lregs lmem lwsrc src v ->
-    unique_in_machineL lregs' lmem' lwsrc src v.
+  Lemma sweep_true_specL (phr : Reg) (phm : Mem) (lr : LReg) (lm : LMem)
+    (cur_map : VMap) (src : RegName) (lwsrc : LWord):
+    lr !! src = Some lwsrc →
+    state_phys_log_corresponds phr phm lr lm cur_map →
+    sweep phm phr src = true →
+    unique_in_machineL lm lr src lwsrc.
   Proof.
   Admitted.
 
-  Lemma not_unique_in_machineL_weaken (lregs lregs' : LReg) (lmem lmem': LMem)
-    p b e a v src:
-    lregs' ⊆ lregs ->
-    lmem' ⊆ lmem ->
-    ¬ unique_in_machineL lregs lmem  (LCap p b e a v) src v ->
-    ¬ unique_in_machineL lregs' lmem' (LCap p b e a v) src v.
+  Lemma sweep_false_specL (phr : Reg) (phm : Mem) (lr : LReg) (lm : LMem)
+    (cur_map : VMap) (src : RegName) (lwsrc : LWord):
+    lr !! src = Some lwsrc →
+    state_phys_log_corresponds phr phm lr lm cur_map →
+    sweep phm phr src = false →
+    not (unique_in_machineL lm lr src lwsrc).
   Proof.
   Admitted.
 
@@ -111,10 +66,10 @@ Section cap_lang_rules.
     lregs !! src = Some lwsrc ->
     get_lcap lwsrc = Some (LSCap p b e a v) ->
     (* check if the words overlap only if the versions matches *)
-    unique_in_machineL lregs lmem lwsrc src v ->
+    unique_in_machineL lmem lregs src lwsrc ->
 
     (* we update the region of memory with the new version *)
-    update_version lmem (finz.seq_between b e) v (v + 1) = Some lmem' ->
+    update_version_word_region lmem lwsrc (v+1) = Some lmem' →
 
     incrementLPC (<[ dst := LInt 1 ]> (<[ src := LCap p b e a (v+1) ]> lregs)) = Some lregs' ->
     IsUnique_spec lregs lmem dst src lregs' lmem' NextIV
@@ -124,7 +79,7 @@ Section cap_lang_rules.
     lregs !! src = Some lwsrc ->
     get_lcap lwsrc = Some (LSCap p b e a v) ->
     (* it exists a word in the memory that overlaps somewhere in the machine *)
-    not (unique_in_machineL lregs lmem lwsrc src v) ->
+    not (unique_in_machineL lmem lregs src lwsrc) ->
     incrementLPC (<[ dst := LInt 0 ]> lregs) = Some lregs' ->
     lmem' = lmem ->
     IsUnique_spec lregs lmem dst src lregs' lmem' NextIV
@@ -143,96 +98,6 @@ Section cap_lang_rules.
                    then Forall (fun a' => exists lw, lmem !! (a',v) = Some lw) (finz.seq_between b e)
                    else True.
 
-
-  (* TODO should it also implies a modification in cur_map ? *)
-  Lemma sweep_true_spec reg mem lr lm cur_map r p b e a v:
-    state_phys_log_corresponds reg mem lr lm cur_map ->
-    sweep mem reg r = true ->
-    reg !! r = Some (WCap p b e a) ->
-    unique_in_machineL lr lm (LCap p b e a v) r v.
-  Proof.
-  Admitted.
-
-
-  Lemma sweep_memory_spec_false (mem : Mem) (regs : Reg) (src : RegName) (wsrc : Word) :
-    sweep_memory mem regs src = false ->
-    regs !! src = Some wsrc ->
-    not (unique_in_memory mem wsrc).
-  Proof.
-    intros Hsweep Hsrc.
-    rewrite /unique_in_memory.
-  Admitted.
-
-  Lemma sweep_false_spec reg mem lr lm cur_map r p b e a v:
-    state_phys_log_corresponds reg mem lr lm cur_map ->
-    sweep mem reg r = false ->
-    lr !! r = Some (LCap p b e a v) ->
-    not (unique_in_machineL lr lm (LCap p b e a v) r v).
-  Proof.
-    intros [HinvReg HinvMem] Hsweep Hlr.
-    assert (reg !! r = Some (WCap p b e a)) as Hr
-      by (eapply reg_phys_log_get_word in Hlr ; eauto).
-    intro HuniqueL.
-    rewrite /unique_in_machineL in HuniqueL.
-    apply andb_false_iff in Hsweep.
-    destruct Hsweep as [Hsweep | Hsweep].
-    - eapply sweep_memory_spec_false in Hsweep; eauto.
-      edestruct (HuniqueL lr lm) as [HuniqueL_mem HuniqueL_reg].
-      1,2:set_solver.
-      clear HuniqueL.
-      apply Hsweep ; clear Hsweep.
-      destruct HinvMem as [Hdom Hroot].
-      assert (is_cur_word (LCap p b e a v) cur_map) as Hcur_lw
-          by (eapply lreg_read_iscur; eauto).
-      rewrite /unique_in_memoryL in HuniqueL_mem.
-      rewrite /unique_in_memory.
-  Admitted.
-
-  (* TODO move stdpp_extra *)
-  Lemma submseteq_incl `{A : Type} (l1 l2 : list A) :
-    l1 ⊆+ l2 -> incl l1 l2.
-  Proof.
-    intros Hsubset ; induction Hsubset.
-  Admitted.
-
-  Lemma mem_eq_implies_allow_access_map:
-    ∀ (lregs : LReg) (lmem : LMem) (r : RegName) (lw : LWord) p b e a v,
-        Forall (λ a' : Addr, ∃ lw0, lmem !! (a', v) = Some lw0) (finz.seq_between b e)
-      → lregs !! r = Some (LCap p b e a v)
-      → allow_access_map_or_true r lregs lmem.
-  Proof.
-    intros lregs lmem r lw p b e a v Hmem Hr.
-    exists p,b,e,a,v; split.
-    - unfold read_reg_inr. by rewrite Hr.
-    - case_decide; done.
-  Qed.
-
-  (* TODO probably misses hypothesis to prove this*)
-  Lemma mem_implies_allow_access_map:
-    ∀ (lregs : LReg) (lmem : LMem) (r : RegName)
-      (pc_a : Addr) pc_v
-      (lw lw' : LWord) p b e a v,
-      (* (if ((a,v) =? (pc_a, pc_v))%la *)
-      (*  then lmem = <[(pc_a, pc_v):=lw]> ∅ *)
-      (*  else lmem = <[(pc_a, pc_v):=lw]> (<[(a, v):=lw']> ∅)) *)
-      (* -> *)
-      Forall (λ a' : Addr, ∃ lw0, lmem !! (a', pc_v) = Some lw0) (finz.seq_between b e)
-      → lregs !! r = Some (LCap p b e a v)
-      → allow_access_map_or_true r lregs lmem.
-  Proof.
-    intros lregs lmem r pc_a pc_v lw lw' p b e a v Hcond Hr.
-    (* apply *)
-    (* destruct ((a,v) =? (pc_a, pc_v))%la eqn:Heq; cbn in Heq. *)
-    (*   + apply andb_true_iff in Heq. destruct Heq as [Heq1 Heq2]. *)
-    (*     apply Z.eqb_eq, finz_to_z_eq in Heq1. subst a. *)
-    (*     apply Nat.eqb_eq in Heq2. subst v. *)
-    (*     eapply mem_eq_implies_allow_access_map; eauto. *)
-    (*   + apply andb_false_iff in Heq. destruct Heq as [Heq | Heq] *)
-    (*   ; [ apply Z.eqb_neq in Heq |  apply Nat.eqb_neq in Heq ] *)
-    (*   ; eapply (mem_neq_implies_allow_access_map _ _ _ pc_a pc_v _ _ _ _ _ a v) ; eauto. *)
-    (*     left ; solve_addr. *)
-   Admitted.
-
   Lemma allow_access_implies_memmap:
     ∀ (r : RegName) (lmem : LMem) (lregs : LReg) (p : Perm) (b e a : Addr) v,
       allow_access_map_or_true r lregs lmem
@@ -247,85 +112,6 @@ Section cap_lang_rules.
     - exact Hmem.
     - contradiction Hrega.
   Qed.
-
-  (* TODO @bastien move *)
-  Definition map_insert_list
-    {L V : Type} {EqDecision0 : EqDecision L}
-    {H : Countable L}
-    (m : gmap L V)
-    (l : list (L*V)) : gmap L V :=
-    foldl (fun mres ins => <[ ins.1 := ins.2]> mres) m l.
-
-  (* TODO instead of =map_insert_list=, maybe I should use something related with
-     update_addr_version_lmem_list and update_addr_version_vmap_list instead ?
-   *)
-  (* TODO @bastien move *)
-  Lemma gen_heap_update_list_inSepM :
-    ∀ {L V : Type} {EqDecision0 : EqDecision L}
-      {H : Countable L} {Σ : gFunctors}
-      {gen_heapG0 : gen_heapGS L V Σ}
-      (σ σ' : gmap L V) (ll : list L) (lv : list V),
-      Forall (fun l => is_Some (σ' !! l)) ll →
-      gen_heap_interp σ
-      -∗ ([∗ map] k↦y ∈ σ', mapsto k (DfracOwn 1) y)
-      ==∗ gen_heap_interp (map_insert_list σ (zip ll lv))
-          ∗ [∗ map] k↦y ∈ (map_insert_list σ' (zip ll lv)), mapsto k (DfracOwn 1) y.
-  Proof.
-    induction ll; intros * Hσ'.
-    - iIntros "Hh H"; cbn.
-      iModIntro.
-      iSplitL "Hh"; eauto.
-    - admit.
-      (* rewrite (big_sepM_delete _ (<[l:=v]> σ') l). *)
-      (* { rewrite delete_insert_delete. iFrame. } *)
-      (* rewrite lookup_insert //. *)
-  Admitted.
-
-  (* TODO ugly lemma, how to get a better one ? *)
-  Lemma insert_update_spec a pc_v v v' lw lregion:
-    forall b e, lregion = logical_region (finz.seq_between b e) v ->
-           ∀ lmem,
-             lmem !! (a, pc_v) = Some lw
-             → Forall (λ a : Addr, ∃ lw0, lmem !! (a, v) = Some lw0) (finz.seq_between b e)
-             → Forall (λ la : LAddr, is_Some (lmem !! la)) lregion
-             → ∀ lv : list LWord,
-                 Forall (λ kv : LAddr * LWord, lmem !! (kv.1.1, v) = Some kv.2)
-                   (zip lregion lv)
-                 → length lv = length lregion
-                 → foldl
-                     (λ (opt_lmem' : option LMem) (la : LAddr),
-                       opt_lmem'
-                         ≫= (λ lmem',
-                              lmem' !! la ≫= (λ lw0, Some (<[(la.1, v'):=lw0]> lmem'))))
-                     (Some lmem) lregion = Some (map_insert_list lmem (zip lregion lv))
-  .
-  Proof.
-    induction lregion as [|la lregion']; intros b e Hlregion lmem Hlapc HmemMap HmemMap_isSome lv Hlv Hlen_lv
-    ; cbn ; auto.
-    destruct lv as [| w lv'] ; [by cbn in Hlen_lv|].
-    cbn in *; simplify_eq.
-    eapply Forall_cons in HmemMap_isSome.
-    destruct HmemMap_isSome as [Hla HmemMap_isSome].
-    eapply Forall_cons in Hlv.
-    destruct Hlv as [Hlmem Hlv]; cbn in *.
-    eapply IHlregion' in HmemMap_isSome;eauto;clear IHlregion'.
-    (* destruct (lmem !! la) as [ a_lw|] eqn:Heq ; [cbn| destruct Hla ; done ]. *)
-    (* replace *)
-    (*   (foldl (λ (mres : gmap LAddr LWord) (ins : LAddr * LWord), <[ins.1:=ins.2]> mres) *)
-    (*      (<[la:=v]> lmem) (zip lregion' lv')) *)
-    (*   with *)
-    (*   (<[la:=v]> (foldl (λ (mres : gmap LAddr LWord) (ins : LAddr * LWord), <[ins.1:=ins.2]> mres) *)
-    (*                 (lmem) (zip lregion' lv'))). *)
-    (* 2: { admit. } *)
-    (* rewrite -/(map_insert_list lmem (zip lregion' lv')). *)
-  Admitted.
-
-  (* TODO It misses hypothesis *)
-  Lemma update_version_spec b e v v' lregion lv lmem:
-    lregion = (λ a : Addr, (a, v')) <$> finz.seq_between b e ->
-    update_version lmem (finz.seq_between b e) v v' =
-      Some (map_insert_list lmem (zip lregion lv)).
-  Admitted.
 
   (* NOTE/TODO: Sum up.
      For the case where is_unique succeed, the specification gives us that,
@@ -346,6 +132,61 @@ Section cap_lang_rules.
     of the addresses/words. From =unique_in_machineL=, we know that it will actually cancel
     nothing else.
    *)
+
+  (* TODO property desired about update_version_word_region *)
+  Lemma update_cur_version_region_implies_next_version
+    (lm lm' : LMem) (cur_map cur_map': VMap)
+    (p : Perm) (b e a : Addr) (v : Version) :
+    is_cur_word (LCap p b e a v) cur_map ->
+    update_cur_version_region lm cur_map (finz.seq_between b e) = Some (lm', cur_map') ->
+    update_version_word_region lm (LCap p b e a v) (v + 1) = Some lm'.
+  Proof.
+  Admitted.
+
+  (* TODO property desired about unique_in_machineL *)
+  Lemma unique_in_machine_monoL
+    (lm lmem : LMem) (lr lregs : LReg) (src : RegName)
+    (p : Perm) (b e a : Addr) (v : Version) :
+    lmem ⊆ lm ->
+    lregs ⊆ lr ->
+    lr !! src = Some (LCap p b e a v) ->
+    unique_in_machineL lm lr src (LCap p b e a v) ->
+    unique_in_machineL lmem lregs src (LCap p b e a v).
+  Proof.
+  Admitted.
+
+  (* TODO property desired about unique_in_machineL *)
+  Lemma unique_in_machine_no_accessL
+    (lm : LMem) (lr : LReg) (cur_map : VMap) (src : RegName)
+    (p : Perm) (b e a : Addr) ( v : Version ) :
+    (is_cur_word (LCap p b e a v) cur_map) ->
+    unique_in_machineL lm lr src (LCap p b e a v) ->
+    Forall
+      (λ a' : Addr, lmem_not_access_addrL lm cur_map a')
+      (finz.seq_between b e).
+  Proof.
+  Admitted.
+
+
+  (* TODO maybe we can have a more general way to update the resources *)
+  Lemma gen_heap_lmem_version_update :
+    ∀ (lm lmem lm' lmem': LMem) (cur_map cur_map': VMap)
+      (b e : Addr) ( v : Version ),
+    update_cur_version_region lm cur_map (finz.seq_between b e) = Some (lm', cur_map') ->
+    update_cur_version_region lmem cur_map (finz.seq_between b e) = Some (lmem', cur_map') ->
+    Forall (λ a : Addr, ∃ lw, lmem !! (a, v) = Some lw) (finz.seq_between b e) ->
+    Forall (λ a : Addr, cur_map !! a = Some v) (finz.seq_between b e) ->
+    (* is_Some (lmem !! la) → *)
+    gen_heap_interp lm
+    -∗ ([∗ map] k↦y ∈ lmem, mapsto k (DfracOwn 1) y)
+    ==∗ gen_heap_interp lm'
+      ∗ [∗ map] k↦y ∈ lmem', mapsto k (DfracOwn 1) y.
+  Proof.
+    iIntros
+      (lm lmem lm' lmem' cur_map cur_map' b e v Hupd_lm Hupd_lmem
+         HmemMap HcurMap)
+        "Hgen Hmem".
+  Admitted.
 
 
   Lemma wp_isunique Ep
@@ -419,10 +260,7 @@ Section cap_lang_rules.
     (* sweep success or sweep fail *)
     destruct (sweep mem reg src) as [|] eqn:Hsweep ; cbn in Hstep.
     - (* sweep is true *)
-
-      (* Derive spec of sweep that returns true -> no overlap *)
-      eapply sweep_true_spec with (v := v) in Hsweep; eauto.
-      eapply unique_in_machineL_weaken in Hsweep; eauto.
+      eapply sweep_true_specL in Hsweep; eauto.
 
       destruct (incrementLPC (<[ dst := LInt 1 ]>
                                 (<[ src := LCap p b e a (v+1)]> lregs)))
@@ -477,62 +315,11 @@ Section cap_lang_rules.
       inversion Hstep; clear Hstep ; simplify_map_eq.
 
       (* we destruct the cases when the registers are equals *)
-      destruct (decide (src = PC)); simplify_map_eq.
-      * (* src = PC *)
-        rewrite (insert_commute _ dst PC) //= insert_insert insert_commute //= in H'lregs'.
-        (* we update the registers with their new value *)
-        iMod ((gen_heap_update_inSepM _ _ dst ) with "Hr Hmap") as "[Hr Hmap]"; eauto.
-        iMod ((gen_heap_update_inSepM _ _ PC ) with "Hr Hmap") as "[Hr Hmap]"; eauto
-        ; first by simplify_map_eq.
-        (* we update the version of the memory region *)
-        set (lregion := (logical_region (finz.seq_between b1 e1) (pc_v+1))).
-
-        assert ( exists (lv : list LWord),
-                   length lv = length lregion /\
-                     Forall (λ (kv : LAddr * LWord),
-                         lmem !! (kv.1.1, pc_v) = Some kv.2)
-                       (zip lregion lv)
-               ) as  (lv & Hlen_lv & Hlv).
-        {  admit. }
-
-        assert (HmemMap_isSome: Forall (λ la : LAddr, is_Some (lmem !! la)) lregion).
-        {  admit. }
-
-        iMod ((gen_heap_update_list_inSepM lm _ _ lv HmemMap_isSome) with "Hm Hmem")
-          as "[Hm Hmem]".
-
-        iFrame; iModIntro ; iSplitR "Hφ Hmap Hmem".
-        2: {
-          iApply "Hφ" ; iFrame; iPureIntro; econstructor; eauto.
-          eapply update_version_spec ; eauto.
-        }
-
-        iExists _, (map_insert_list lm (zip lregion lv)), cur_map; iFrame; auto
-        ; iPureIntro; econstructor; eauto
-        ; destruct HLinv as [[Hstrips Hcur_reg] [Hdom Hroot]]
-        ; cbn in *.
-        split; first by rewrite -Hstrips /lreg_strip !fmap_insert /=.
-        apply map_Forall_insert_2.
-        2: apply map_Forall_insert_2; cbn ; auto.
-        intros a Hbounds_a.
-        (* eapply map_Forall_lookup_1 ; eauto. *)
-        admit.
-        (* TODO need a lemma with map_insert_list for mem_phys_log *)
-        (* TODO I think that I also need a lemma that bumps the version of the
-       addresses in cur_map, but probably before *)
-        split; eauto.
-        admit.
-        admit.
-
+      destruct (decide (src = PC)); simplify_map_eq ; cycle 1.
       * (* src <> PC *)
-        (* TODO also need to destruct on (dst = src) *)
-
         destruct (decide (src = dst)) ; simplify_map_eq.
         ** (* src = dst *) admit.
         ** (* src <> dst *)
-
-
-
           iMod ((gen_heap_update_inSepM _ _ src (LCap p b e a (v + 1))) with "Hr Hmap")
             as "[Hr Hmap]"; eauto.
           iMod ((gen_heap_update_inSepM _ _ dst (LInt 1)) with "Hr Hmap")
@@ -540,88 +327,91 @@ Section cap_lang_rules.
           iMod ((gen_heap_update_inSepM _ _ PC (LCap p1 b1 e1 a_pc1 v1)) with "Hr Hmap")
             as "[Hr Hmap]"; eauto ; first by simplify_map_eq.
 
-        (* we update the version of the memory region *)
-        set (lregion := (logical_region (finz.seq_between b e) (v+1))).
+          assert (HcurMap : Forall (λ a0 : Addr, cur_map !! a0 = Some v) (finz.seq_between b e)).
+          { admit. (* should be a consequence of HLinv and HmemMap *) }
 
-        assert ( exists (lv : list LWord),
-                   length lv = length lregion /\
-                     Forall (λ (kv : LAddr * LWord), lmem !! (kv.1.1, v) = Some kv.2)
-                       (zip lregion lv)
-               ) as  (lv & Hlen_lv & Hlv).
-        {  admit. }
+          assert (HNoDup : NoDup (finz.seq_between b e)) by (apply finz_seq_between_NoDup).
 
-        assert (HmemMap_isSome: Forall (λ la : LAddr, is_Some (lmem !! la)) lregion).
-        {  admit. }
+          destruct (update_cur_version_word_region lmem cur_map (LCap p b e a v))
+            as [[lmem' cur_map']|] eqn:Hupd_lm
+          ; rewrite /update_cur_version_word_region /= in Hupd_lm.
+          {
+            Set Nested Proofs Allowed.
 
-        iMod ((gen_heap_update_list_inSepM lm _ _ lv HmemMap_isSome) with "Hm Hmem")
-          as "[Hm Hmem]".
 
-        iFrame; iModIntro ; iSplitR "Hφ Hmap Hmem".
-        2: {
-          iApply "Hφ" ; iFrame; iPureIntro; econstructor; eauto.
-          eapply update_version_spec ; eauto.
-        }
+            pose proof Hupd_lm as Hupd_lmem.
+            eapply update_cur_version_region_mono in Hupd_lmem ; eauto.
+            destruct Hupd_lmem as (lm' & Hupd_lmem & Hmem').
 
-        iExists _, (map_insert_list lm (zip lregion lv)), cur_map; iFrame; auto
-        ; iPureIntro; econstructor; eauto
-        ; destruct HLinv as [[Hstrips Hcur_reg] [Hdom Hroot]]
-        ; cbn in *.
-        split; first rewrite -Hstrips /lreg_strip !fmap_insert /=.
-        replace (<[src:=WCap p b e a]> ((λ lw0, lword_get_word lw0) <$> lr))
-                  with ((λ lw0, lword_get_word lw0) <$> lr); first done.
-        { replace (WCap p b e a) with (lword_get_word (LCap p b e a v)) by auto.
-        rewrite <- fmap_insert, insert_id; auto.
-        }
 
-        apply map_Forall_insert_2.
-        2: apply map_Forall_insert_2; cbn ; auto.
-        intros a' Hbounds_a'.
-        (* eapply map_Forall_lookup_1 ; eauto. *)
+            iMod ((gen_heap_lmem_version_update lm lmem lm' lmem' ) with "Hm Hmem")
+              as "[Hm Hmem]"; eauto.
+
+            iFrame; iModIntro ; iSplitR "Hφ Hmap Hmem".
+            2: {
+              iApply "Hφ" ; iFrame; iPureIntro; econstructor; eauto.
+              by eapply unique_in_machine_monoL.
+              eapply update_cur_version_region_implies_next_version; eauto.
+              destruct HLinv as [Hinv_reg _].
+              eapply lreg_read_iscur; eauto.
+            }
+            {
+              rewrite /state_interp_logical.
+              iExists _, lm', cur_map'; iFrame; auto
+              ; iPureIntro; econstructor; eauto
+              ; destruct HLinv as [[Hstrips Hcur_reg] [Hdom Hroot]]
+              ; cbn in *.
+              { admit . }
+              eapply update_cur_version_region_preserves_mem_phyc_cor; eauto.
+              eapply unique_in_machine_no_accessL ; eauto.
+              split ; auto.
+            }
+          }
+          {
+            exfalso.
+            apply eq_None_not_Some in Hupd_lm.
+            apply Hupd_lm.
+            eapply update_cur_version_region_Some; eauto.
+          }
+
+      * (* src = PC *)
+        rewrite (insert_commute _ dst PC) //= insert_insert insert_commute //= in H'lregs'.
+        (* we update the registers with their new value *)
+        iMod ((gen_heap_update_inSepM _ _ dst ) with "Hr Hmap") as "[Hr Hmap]"; eauto.
+        iMod ((gen_heap_update_inSepM _ _ PC ) with "Hr Hmap") as "[Hr Hmap]"; eauto
+        ; first by simplify_map_eq.
+
+       (*  (* we update the version of the memory region *) *)
+       (*  iMod ((gen_heap_update_list_inSepM lm _ _ lv HmemMap_isSome) with "Hm Hmem") *)
+       (*    as "[Hm Hmem]". *)
+
+       (*  iFrame; iModIntro ; iSplitR "Hφ Hmap Hmem". *)
+       (*  2: { *)
+       (*    iApply "Hφ" ; iFrame; iPureIntro; econstructor; eauto. *)
+       (*    eapply update_version_spec ; eauto. *)
+       (*  } *)
+
+       (*  iExists _, (map_insert_list lm (zip lregion lv)), cur_map; iFrame; auto *)
+       (*  ; iPureIntro; econstructor; eauto *)
+       (*  ; destruct HLinv as [[Hstrips Hcur_reg] [Hdom Hroot]] *)
+       (*  ; cbn in *. *)
+       (*  split; first by rewrite -Hstrips /lreg_strip !fmap_insert /=. *)
+       (*  apply map_Forall_insert_2. *)
+       (*  2: apply map_Forall_insert_2; cbn ; auto. *)
+       (*  intros a Hbounds_a. *)
+       (*  (* eapply map_Forall_lookup_1 ; eauto. *) *)
+       (*  admit. *)
+       (*  (* TODO need a lemma with map_insert_list for mem_phys_log *) *)
+       (*  (* TODO I think that I also need a lemma that bumps the version of the *)
+       (* addresses in cur_map, but probably before *) *)
+       (*  split; eauto. *)
+       (*  admit. *)
+       (*  admit. *)
         admit.
-        (* TODO need a lemma with map_insert_list for mem_phys_log *)
-        (* TODO I think that I also need a lemma that bumps the version of the
-       addresses in cur_map, but probably before *)
-        (* TODO the kind of lemma would be:
-           IF:
-           - map_Forall (λ (_ : RegName) lw, is_cur_word lw cur_map) lr
-           - map_Forall (λ (la : LAddr) (_ : LWord), is_cur_addr la cur_map) lm
-           - map_Forall
-              (λ (a : Addr) v,
-               ∃ lw,
-                 lm !! (a, v) = Some lw
-                 ∧ mem !! a = Some (lword_get_word lw) ∧ is_cur_word lw cur_map) cur_map
-            THEN:
-            =we update the version of a word w=: update_version w cur_map
-            =the previous invariant holds with the new cur_map, modification in
-            logical memory / registers=
-
-    ---------------------- ----------------------
-
-        Example for lregs:
-
-        - lr !! src = Some (LCap p b e a v)
-        - map_Forall (λ (_ : RegName) lw, is_cur_word lw cur_map) lr
-          ->
-         map_Forall
-         (λ (_ : RegName) lw, is_cur_word lw (update_vmap (range b e) v' cur_map))
-         (<[src:=LCap p b e a v']> lr)
-
-        Similar lemmas for lmem:
-        - update one address
-        - update a whole region
-
-         *)
-        (* split; eauto. *)
-        admit.
-        admit.
-
-
 
     - (* sweep = false *)
 
-      eapply sweep_false_spec with (v := v) in Hsweep ; [|eauto|eauto].
-      eapply not_unique_in_machineL_weaken in Hsweep ; eauto.
-
+      eapply sweep_false_specL in Hsweep; eauto.
       destruct (incrementLPC (<[ dst := LInt 0 ]> lregs))
         as  [ lregs' |] eqn:Hlregs'
       ; pose proof Hlregs' as H'lregs'
@@ -673,7 +463,17 @@ Section cap_lang_rules.
       ; first by simplify_map_eq.
 
       iFrame; iModIntro ; iSplitR "Hφ Hmap Hmem".
-      2: { iApply "Hφ" ; iFrame; iPureIntro; eapply IsUnique_success_false; eauto. }
+      2: { iApply "Hφ" ; iFrame; iPureIntro. ; eapply IsUnique_success_false ; eauto.
+           (* TODO intuitively, this is not true...
+              because lm is the global (authoritative) memory,
+              while lmem is the local (fragmental) memory.
+              But what could happen is that,
+              there is a word overlapping with [b,e) in `lm`
+              which is not in `lmem`.
+              How to deal with this ?
+            *)
+           admit.
+      }
 
       iExists _, lm, cur_map; iFrame; auto
       ; iPureIntro; econstructor; eauto
